steel/Zeta.Steel.AggregateEpochHashes.fsti
@@ -1,0 +1,102 @@
+module Zeta.Steel.AggregateEpochHashes
+
+open FStar.Ghost
+open Zeta.Steel.ApplicationTypes
+module U8 = FStar.UInt8
+module U16 = FStar.UInt16
+module U32 = FStar.UInt32
+module U64 = FStar.UInt64
+open Zeta.Steel.FormatsManual
+open Steel.Memory
+open Steel.Effect.Atomic
+open Steel.Effect
+open Steel.Reference
+open Steel.Array
+module IArray = Steel.Hashtbl
+module T = Zeta.Steel.FormatsManual
+module M = Zeta.Steel.ThreadStateModel
+module A = Steel.Array
+module Lock = Steel.SpinLock
+module HA = Zeta.Steel.HashAccumulator
+#push-options "--ide_id_info_off"
+
+val epoch_hash_size : U32.t
+
+let log_ref = ghost_ref (Seq.seq log_entry_base)
+
+let log_refs_t = Map.t thread_id log_ref
+
+let hash_value = u256 & U64.t
+let zero_hash : HA.hash_value_t = admit()
+let related_hashes (h:hash_value) (h':HA.hash_value_t) = True // TODO
+
+noeq
+type epoch_hash_t = {
+  hadd: hash_value;
+  hevict: hash_value;
+  certified: bool;
+}
+
+let related (h h':M.epoch_hash) =
+   (if h'.epoch_complete
+    then h == h'
+    else (
+      h.hadd == zero_hash /\
+      h.hevict == zero_hash
+   ))
+
+let epoch_id_hash = fun (e:M.epoch_id) -> e
+let epoch_hashes_t = IArray.tbl M.epoch_id epoch_hash_t epoch_id_hash
+let epoch_hash_contributions_t = Map.t (thread_id & M.epoch_id) M.epoch_hash
+
+let all_contributions_are_accurate (_:IArray.repr M.epoch_id epoch_hash_t)
+                                   (_:epoch_hash_contributions_t)
+  : prop
+  = True //TODO
+
+let max_certified_epoch_is (_:IArray.repr M.epoch_id epoch_hash_t)
+                           (_:M.epoch_id)
+  : prop
+  = True //TODO
+
+let per_thread_contribiution_is_accurate (tid:thread_id)
+                                         (entries:Seq.seq log_entry_base)
+                                         (contribs:epoch_hash_contributions_t)
+  : prop
+  = let tsm = M.verify_model (M.init_thread_state_model tid) entries in
+    forall (eid:M.epoch_id). related (Map.sel contribs (tid, eid))
+                                (Map.sel tsm.epoch_hashes eid)
+
+let full = Steel.FractionalPermission.full_perm
+let half = Steel.FractionalPermission.half_perm full
+val h_forall (#a:Type u#a) (f: a -> vprop) : vprop
+
+let lock_inv (log_refs:log_refs_t)
+             (hashes : epoch_hashes_t)
+             (max_certified_epoch : ref M.epoch_id)
+             (contributions: ghost_ref epoch_hash_contributions_t)
+ : vprop
+ = h_exists (fun (hashes_v, max, contributions_v) ->
+      IArray.tpts_to hashes hashes_v `star`
+      pts_to max_certified_epoch full max `star`
+      ghost_pts_to contributions full contributions_v `star`
+      pure (all_contributions_are_accurate hashes_v contributions_v /\
+            max_certified_epoch_is hashes_v max) `star`
+      h_forall (fun (tid:thread_id) ->
+        if Map.contains log_refs tid
+        then (
+          let logref = Map.sel log_refs tid in
+          h_exists (fun (entries:_) ->
+            ghost_pts_to logref half entries `star`
+            pure (per_thread_contribiution_is_accurate tid entries contributions_v))
+        )
+        else emp
+      ))
+
+noeq
+type aggregate_epoch_hashes (log_refs:log_refs_t) = {
+     hashes : epoch_hashes_t;
+     max_certified_epoch : ref M.epoch_id;
+     contributions: ghost_ref epoch_hash_contributions_t;
+     lock: Lock.lock (lock_inv log_refs hashes max_certified_epoch contributions)
+}
