steel/Zeta.Steel.Main.fsti
@@ -1,0 +1,170 @@
+module Zeta.Steel.Main
+open FStar.Ghost
+open Zeta.Steel.ApplicationTypes
+module U8 = FStar.UInt8
+module U16 = FStar.UInt16
+module U32 = FStar.UInt32
+module U64 = FStar.UInt64
+open Zeta.Steel.FormatsManual
+open Steel.Memory
+open Steel.Effect.Atomic
+open Steel.Effect
+open Steel.Reference
+open Steel.Array
+
+module T = Zeta.Steel.FormatsManual
+module M = Zeta.Steel.ThreadStateModel
+module A = Steel.Array
+module AEH = Zeta.Steel.AggregateEpochHashes
+module V = Zeta.Steel.Verifier
+module Lock = Steel.SpinLock
+module SA = Zeta.SeqAux
+module MR = Steel.MonotonicReference
+#push-options "--ide_id_info_off"
+val thread_state_pts_to (t:V.thread_state_t)
+                        (tsm:M.thread_state_model)
+  : vprop
+
+let grows (#a:Type) :Preorder.preorder (erased (Seq.seq a))
+  = let open FStar.Seq in
+    fun (s1 s2:erased (seq a)) ->
+      length s1 <= length s2 /\
+      (forall (i:nat).{:pattern (Seq.index s1 i) \/ (Seq.index s2 i)}
+         i < length s1 ==> index s1 i == index s2 i)
+
+let log = Seq.seq log_entry_base
+let elog = erased log
+
+/// This should be a MR.ghost_ref
+let monotonic_log_t = MR.ref elog grows
+
+let mlog_refs_t = Map.t thread_id monotonic_log_t
+
+let thread_inv (t: V.thread_state_t)
+               (logref: AEH.log_ref)
+               (mlogref: monotonic_log_t)
+  : vprop
+  = h_exists (fun (tsm, committed_entries) ->
+       thread_state_pts_to t tsm `star`
+       ghost_pts_to logref AEH.half committed_entries `star`
+       MR.pts_to mlogref AEH.half tsm.M.processed_entries `star`
+       pure (V.committed_prefix tsm.M.processed_entries committed_entries))
+
+noeq
+type thread_state (logrefs:AEH.log_refs_t)
+                  (mlogrefs:mlog_refs_t) =
+{
+  tid: tid;
+  tsm: V.thread_state_t;
+  logref: AEH.log_ref;
+  mlogref: monotonic_log_t;
+  lock : Lock.lock (thread_inv tsm logref mlogref);
+  properties : squash (
+    logref == Map.sel logrefs tid /\
+    mlogref == Map.sel mlogrefs tid
+  );
+}
+
+let all_threads_t logrefs mlogrefs =
+  a:A.array (thread_state logrefs mlogrefs) {
+      A.length a == U32.v n_threads
+  }
+
+noeq
+type top_level_state = {
+  logrefs : erased AEH.log_refs_t;
+  mlogrefs : erased mlog_refs_t; //should be erased
+  all_threads : all_threads_t logrefs mlogrefs;
+  epoch_hashes: AEH.aggregate_epoch_hashes logrefs;
+}
+
+val array_pts_to (#t:Type0)
+                 (a:A.array t)
+                 (p:Steel.FractionalPermission.perm)
+                 (v:Seq.lseq t (A.length a))
+  : vprop
+
+let tid_positions_ok #l #m (all_threads: Seq.seq (thread_state l m))
+  : prop
+  = forall (i:SA.seq_index all_threads).
+        let si = Seq.index all_threads i in
+        U16.v si.tid == i
+
+let core_inv (t:top_level_state)
+  : vprop
+  = h_exists (fun (perm, v) ->
+      array_pts_to t.all_threads perm v `star`
+      pure (tid_positions_ok v))
+
+let initial_inv (t:top_level_state)
+  : vprop
+  = core_inv t `star`
+    AEH.h_forall (fun (tid:thread_id) ->
+      if Map.contains t.mlogrefs tid
+      then MR.pts_to (Map.sel t.mlogrefs tid) AEH.half Seq.empty
+      else emp)
+
+val init (_:unit)
+  : SteelT top_level_state emp initial_inv
+
+val verify_entries (t:top_level_state)
+                   (tid:thread_id)
+                   (len: U32.t) (input:A.array U8.t { A.length input == U32.v len })
+                   (out_len: U32.t) (output:A.array U8.t { A.length output == U32.v out_len })
+                   (entries:erased (Seq.seq log_entry_base))
+                   (mlogref:monotonic_log_t)
+  : Steel (bool & U32.t & erased (Seq.seq log_entry_base))
+    (core_inv t `star`
+     A.varray input `star`
+     A.varray output `star`
+     MR.pts_to mlogref AEH.half entries)
+    (fun res ->
+      core_inv t `star`
+      A.varray input `star`
+      A.varray output `star`
+      MR.pts_to mlogref AEH.half (let _, _, e = res in e))
+    (requires fun _ ->
+      Map.sel t.mlogrefs tid == mlogref)
+    (ensures fun h0 (b, n, e) h1 ->
+      let out_bytes = A.asel output h1 in
+      if b
+      then match V.spec_parser_log (A.asel input h0) with
+           | Some (entries', _) ->
+             let tsm0 = M.verify_model (M.init_thread_state_model tid) entries in
+             let tsm1 = M.verify_model tsm0 entries' in
+             e == hide (Seq.append entries entries') /\
+             V.serialized_new_app_results tsm0.app_results tsm1.app_results n out_bytes
+           | _ ->
+             True
+      else True)
+
+let prefix_of (#a:Type) (s0 s1:Seq.seq a)
+  : prop
+  = let open FStar.Seq in
+    length s0 <= length s1 /\
+    Seq.slice s1 0 (length s0) == s0
+
+let snapshot (r:monotonic_log_t) (s:log) =
+  MR.witnessed r (fun s' -> prefix_of s s')
+
+let run_threads (logs:(Map.t tid log)) (tid:tid)
+  : M.thread_state_model
+  = M.verify_model (M.init_thread_state_model tid) (Map.sel logs tid)
+
+val verified_and_epoch_hash_ok (logs:Map.t tid log) (eid:M.epoch_id) : prop //TODO
+
+val max_certified_epoch (t:top_level_state)
+                        (entries: erased (Map.t tid log))
+  : Steel M.epoch_id
+    (core_inv t)
+    (fun _ -> core_inv t)
+    (requires fun _ ->
+      forall (tid:tid). let lr_i = Map.sel t.mlogrefs tid in
+                   snapshot lr_i (Map.sel entries tid))
+    (ensures fun _ max _ ->
+      forall (eid:M.epoch_id).
+         U32.v eid <= U32.v max ==>
+         //From this, we should connect back to the semantic
+         //proof and show that the entries are sequentially consistent up to eid
+         //except for hash collisions
+         verified_and_epoch_hash_ok entries eid)
